PhiCalculus.lean
@@ -1,6 +1,14 @@
 import Minimal.Calculus
+import Std.Tactic.Lint
 
 def main : IO Unit :=
   IO.println "Lean 4!"
 
-#eval main
+#lint only checkType checkUnivs defLemma dupNamespace explicitVarsOfIff impossibleInstance nonClassInstance simpComm simpNF simpVarHead synTaut unusedHavesSuffices in Minimal
+
+
+-- #list_linters
+-- rest of linters:
+-- docBlame (*)
+-- docBlameThm
+-- unusedArguments (*)
